src/ExtLib_Monad.v
@@ -1,0 +1,85 @@
+Require Import ExtLib_Any.
+Require Import ExtLib_Functor.
+Require Import ExtLib_Applicative.
+
+Set Implicit Arguments.
+Set Strict Implicit.
+Set Universe Polymorphism.
+
+Class Monad@{d c} (m : Type@{d} -> Type@{c}) : Type :=
+{ ret : forall {t : Type@{d}}, t -> m t
+; bind : forall {t u : Type@{d}}, m t -> (t -> m u) -> m u
+}.
+
+Section monadic.
+
+  Definition liftM@{d c}
+              {m : Type@{d} -> Type@{c}}
+              {M : Monad m}
+              {T U : Type@{d}} (f : T -> U) : m T -> m U :=
+    fun x => bind x (fun x => ret (f x)).
+
+  Definition liftM2@{d c}
+              {m : Type@{d} -> Type@{c}}
+              {M : Monad m}
+              {T U V : Type@{d}} (f : T -> U -> V) : m T -> m U -> m V :=
+    Eval cbv beta iota zeta delta [ liftM ] in
+      fun x y => bind x (fun x => liftM (f x) y).
+
+  Definition liftM3@{d c}
+              {m : Type@{d} -> Type@{c}}
+              {M : Monad m}
+              {T U V W : Type@{d}} (f : T -> U -> V -> W) : m T -> m U -> m V -> m W :=
+    Eval cbv beta iota zeta delta [ liftM2 ] in
+      fun x y z => bind x (fun x => liftM2 (f x) y z).
+
+  Definition apM@{d c}
+              {m : Type@{d} -> Type@{c}}
+              {M : Monad m}
+              {A B : Type@{d}} (fM:m (A -> B)) (aM:m A) : m B :=
+    bind fM (fun f => liftM f aM).
+
+  (* Left-to-right composition of Kleisli arrows. *)
+  Definition mcompose@{c d}
+             {m:Type@{d}->Type@{c}}
+             {M: Monad m}
+             {T U V:Type@{d}}
+             (f: T -> m U) (g: U -> m V): (T -> m V) :=
+    fun x => bind (f x) g.
+
+End monadic.
+
+Module MonadNotation.
+
+  Delimit Scope monad_scope with monad.
+
+  Notation "c >>= f" := (@bind _ _ _ _ c f) (at level 58, left associativity) : monad_scope.
+  Notation "f =<< c" := (@bind _ _ _ _ c f) (at level 61, right associativity) : monad_scope.
+  Notation "f >=> g" := (@mcompose _ _ _ _ _ f g) (at level 61, right associativity) : monad_scope.
+
+  Notation "x <- c1 ;; c2" := (@bind _ _ _ _ c1 (fun x => c2))
+    (at level 61, c1 at next level, right associativity) : monad_scope.
+
+  Notation "e1 ;; e2" := (_ <- e1%monad ;; e2%monad)%monad
+    (at level 61, right associativity) : monad_scope.
+
+  Notation "' pat <- c1 ;; c2" :=
+    (@bind _ _ _ _ c1 (fun x => match x with pat => c2 end))
+    (at level 61, pat pattern, c1 at next level, right associativity) : monad_scope.
+
+End MonadNotation.
+
+Section Instances.
+
+Universe d c.
+Context (m : Type@{d} -> Type@{c}) {M : Monad m}.
+
+Global Instance Functor_Monad@{} : Functor m :=
+{ fmap := @liftM _ _ }.
+
+Global Instance Applicative_Monad@{} : Applicative m :=
+{ pure := @ret _ _
+; ap := @apM _ _
+}.
+
+End Instances.
