src/Test_Extract.v
@@ -1,0 +1,9 @@
+Require Extraction.
+
+Require Import Impl_vm.
+
+Extraction Language CakeML.
+
+(*
+Recursive Extraction copland_compile.
+*)
