src/Test_Extract_App.v
@@ -1,0 +1,8 @@
+Require Extraction.
+
+Require Import Impl_appraisal.
+
+Extraction Language CakeML.
+
+
+Recursive Extraction build_app_comp_evC.
