src/do_coqcpath.sh
@@ -1,0 +1,1 @@
+export PATH="/Users/adampetz/Documents/Summer_2021/coq/_build/install/default/bin:$PATH"
